\section{Additional Exercise 2}
Eigendecomposition of $\bm{V}$ gives us $\bm{V} = \bm{Q}\bm{\Lambda}\bm{Q}^{-1}$ with $\bm{\Lambda} = 
\begin{bmatrix}
\lambda_{1} & &\\
 & \ddots & \\
 &  & \lambda_{p}
\end{bmatrix}$ where $\lambda_{i}$'s are eigenvalues.\\
Since $\bm{V}$ is real symmetric matrix, $\bm{Q}$ is orthogonal matrix (i.e. $\bm{Q}^{-1} = \bm{Q}^{\rm T}$, $\bm{Q}^{\rm T}\bm{Q} = \bm{Q}\bm{Q}^{\rm T} = \bm{I}$).

Because $\bm{V}$ is positive definite, all eigenvalues $\lambda_{1}, \cdots, \lambda_{p}$ are positive. We define
\begin{align*}
\bm{\Lambda}^{\frac{1}{2}} = 
\begin{bmatrix}
\sqrt{\lambda_{1}} & &\\
 & \ddots & \\
 &  & \sqrt{\lambda_{p}}
\end{bmatrix}
\quad \mbox{and} \quad
\bm{\Lambda}^{-\frac{1}{2}} = 
\begin{bmatrix}
\frac{1}{\sqrt{\lambda_{1}}} & &\\
 & \ddots & \\
 &  & \frac{1}{\sqrt{\lambda_{p}}}
\end{bmatrix}.
\end{align*}
Then, $\bm{\Lambda}^{\frac{1}{2}}\bm{\Lambda}^{\frac{1}{2}}  = \bm{\Lambda}$ and $\bm{\Lambda}^{-\frac{1}{2}}\bm{\Lambda}^{-\frac{1}{2}}  = \bm{I}$.\\
Now we define
$\bm{V}^{\frac{1}{2}} = \bm{Q}\bm{\Lambda}^{\frac{1}{2}}\bm{Q}^{\rm T}$ and $\bm{V}^{-\frac{1}{2}} = \bm{Q}\bm{\Lambda}^{-\frac{1}{2}}\bm{Q}^{\rm T}$.


Note that $\bm{V}^{\frac{1}{2}}$ and $\bm{V}^{-\frac{1}{2}}$ are symmetric, and $\bm{V}^{\frac{1}{2}}\bm{V}^{-\frac{1}{2}} = \bm{I}$. So, $\bm{V}^{-\frac{1}{2}} = \left(\bm{V}^{\frac{1}{2}}\right)^{-1}$. Further, $\bm{V}^{\frac{1}{2}}\bm{V}^{\frac{1}{2}} = \bm{V}$.

\subsection*{(a)}
We perform variable transformation $\bm{Z} = \bm{V}^{-\frac{1}{2}}(\bm{Y} - \bm{\mu})$ which gives $\bm{Z} \sim N\left(\bm{0}, \bm{V}^{-\frac{1}{2}}\bm{V}\left(\bm{V}^{-\frac{1}{2}}\right)^{\rm T} \right) = N\left(\bm{0}, \bm{I}\right)$.\\

Thus, we have
\begin{align*}
(\bm{Y} - \bm{\mu})^{\rm T}\bm{V}^{-1}(\bm{Y} - \bm{\mu})
&= (\bm{Y} - \bm{\mu})^{\rm T} \left(\bm{V}^{-\frac{1}{2}}\right)^{\rm T}\bm{V}^{-\frac{1}{2}} (\bm{Y} - \bm{\mu})\\
&= \left(\bm{V}^{-\frac{1}{2}}(\bm{Y} - \bm{\mu})\right)^{\rm T}\left(\bm{V}^{-\frac{1}{2}}(\bm{Y} - \bm{\mu})\right)\\
&= \bm{Z}^{\rm T}\bm{Z}\\
&= \sum_{i=1}^{p} Z_{i}^2\\
&\sim \chi_{p}^2.
\end{align*}

\subsection*{(b)}
We perform variable transformation $\bm{Z} = \bm{V}^{-\frac{1}{2}}\bm{Y}$ which gives $\bm{Z} \sim N\left(\bm{V}^{-\frac{1}{2}}\bm{\mu}, \bm{V}^{-\frac{1}{2}}\bm{V}\left(\bm{V}^{-\frac{1}{2}}\right)^{\rm T} \right) = N\left(\bm{V}^{-\frac{1}{2}}\bm{\mu}, \bm{I}\right)$.\\

Thus, we have
\begin{align*}
\bm{Y}^{\rm T}\bm{V}^{-1}\bm{Y}
&= \bm{Y}^{\rm T} \left(\bm{V}^{-\frac{1}{2}}\right)^{\rm T}\bm{V}^{-\frac{1}{2}}\bm{Y}\\
&= \left(\bm{V}^{-\frac{1}{2}}\bm{Y}\right)^{\rm T}\left(\bm{V}^{-\frac{1}{2}}\bm{Y} \right)\\
&= \bm{Z}^{\rm T}\bm{Z}\\
&= \sum_{i=1}^{p} Z_{i}^2\\
&\sim \chi_{p,\lambda}^2
\end{align*}
where $\lambda = \sum_{i=1}^{p} \E[Z_{i}]^2 = \left(\bm{V}^{-\frac{1}{2}}\bm{\mu}\right)^{\rm T}\left(\bm{V}^{-\frac{1}{2}}\bm{\mu} \right) = \bm{\mu}^{\rm T}\bm{V}^{-1}\bm{\mu}$.