\section*{Additional Exercise 9}
\subsection*{(a)}
Example 1: Bernoulli distribution\\
Example 2: Poisson distribution\\

\subsection*{(b)}
Exponential dispersion family: $f(y) = \exp\left[\frac{\theta y - b(\theta)}{a(\phi)} + c(y,\phi)\right]$\\
If we set $a(\phi) = 1$ and $c(y,\phi) = \log h(y)$, we get $f(y) = h(y)\exp\left[\theta y -b(\theta)\right]$, which is density of natural exponential family.


\subsection*{(c)}
First, note that $1 = \int f(y) \,dy = \int h(y)\exp\left[\theta y -b(\theta)\right] \,dy$. Now we write
\begin{align*}
M_{Y}(t) &= \E\left[e^{Yt}\right]\\
&= \int e^{ty} f(y) \,dy\\
&= \int e^{ty} h(y)\exp\left[\theta y -b(\theta)\right] \,dy\\
&= \int e^{ty} h(y)\exp\left[\theta y + b(\theta + t) - b(\theta + t) -b(\theta)\right] \,dy\\
&= e^{b(\theta + t) -b(\theta)}\int e^{ty} h(y)\exp\left[\theta y -b(\theta + t)\right] \,dy\\
&= e^{b(\theta + t) -b(\theta)}\int h(y)\exp\left[(\theta +t)y -b(\theta + t)\right] \,dy\\
&= e^{b(\theta + t) -b(\theta)}
\end{align*}
Further, $R_{Y}(t) = \log M_{Y}(t) = b(\theta + t) -b(\theta)$.\\
In discrete case, replace the integral by a sum. The result stays same.

\subsection*{d)}
From previous part, we have $R_{Y}(t) = b(\theta + t) -b(\theta)$.
So, $R_{Y}'(t) = b'(\theta + t)$ and $R_{Y}''(t) = b''(\theta + t)$. By combining this with the fact that $\E[Y] = R_{Y}'(0)$ and $\Var[Y] = R_{Y}''(0)$, we get $\E[Y] = b'(\theta)$ and  $\Var[Y] = b''(\theta)$.
