\section*{Additional Exercise 4}

\subsection*{(a)}

The multivariate normal has density
\[
f(x;\mu,\Sigma)=\frac{1}{\sqrt{2\pi\det(\Sigma)}}e^{-\frac{1}{2}(x-\mu)^{T}\Sigma^{-1}(x-\mu)},
\]
see e.g. Wikipedia. When $\Sigma=I\sigma^{2},$the inverse $\Sigma^{-1}=I\sigma^{-2}$
and $\det(\Sigma)=\sigma^{2n}$. It follows that
\begin{eqnarray*}
f(x;\mu,\Sigma) & = & \frac{1}{\sqrt{2^{n}\pi^{n}\det(\sigma^{2n})}}e^{-\frac{1}{2}(x-\mu)^{T}\Sigma^{-1}(x-\mu)},\\
 & = & (2\pi)^{-n/2}\sigma^{-n}e^{-\frac{1}{2\sigma^{2}}(x-\mu)^{T}(x-\mu)},
\end{eqnarray*}
and we are done.

\subsection*{(b)}
Take the logarithm and find that
\begin{eqnarray*}
\log(f(x;\mu,\sigma)) & = & \log(2^{-n/2}\pi^{-n/2}\sigma^{-n})-\frac{1}{2\sigma^{2}}(x-\mu)^{T}\Sigma^{-1}(x-\mu),\\
 & = & -\frac{n}{2}\log2\pi-n\log\sigma-\frac{1}{2\sigma^{2}}(x-\mu)^{T}(x-\mu).
\end{eqnarray*}
Keeping $\sigma$ fixed, 
\[
\log(f(x;\mu,\sigma))=C(\sigma)-\frac{1}{2\sigma^{2}}(x-\mu)^{T}(x-\mu),
\]
where $C(\sigma)$ is independent of $\mu$. Minimizing $(x-\mu)^{T}(x-\mu)$
with respect to $\mu$ is equivalent to least squares, so $\hat{\mu}$is
the least squares solution.

\subsection*{(c)}
Differentiate the expression in (b), using $SSE=(x-\mu)^{T}(x-\mu)$,
\[
\frac{d}{d\mu}(-n\log\sigma-\sigma^{-2}SSE)=-n\sigma^{-1}+\sigma^{3}SSE.
\]
Set it equal to $0$, and
\begin{eqnarray*}
-n\sigma^{-1}+\sigma^{3}SSE & = & 0
\end{eqnarray*}
implies
\[
\sigma^{3}SSE=-n\sigma^{-1},
\]
so that
\[
\hat{\sigma}^{2}=SSE/n.
\]


\subsection*{(d)}
Since $\hat{\sigma}=SSE/n$ , we get
\begin{eqnarray*}
\log l(\hat{\mu},\hat{\sigma}) & = & -\frac{n}{2}\log(2\pi)-n\log\hat{\sigma}-\frac{1}{2}\hat{\sigma}^{-2}SSE,\\
 & = & -\frac{n}{2}\log(2\pi)-n\log\hat{\sigma}-\frac{n}{2}.
\end{eqnarray*}
Exponentiate to get 
\[
l(\hat{\mu},\hat{\sigma})=(2\pi)^{-n/2}\hat{\sigma}^{-n}e^{-n/2}.
\]

\subsection*{(e)}
Let $SSE_{0}$ belong to $X_{0}$ and $SSE_{1}$ belong to $X_{1}$.
Using the result in (d), 
\begin{eqnarray*}
\log l(\hat{\mu}_{0},\hat{\sigma}_{0})-\log l(\hat{\mu}_{1},\hat{\sigma}_{1}) & = & -\frac{n}{2}\log(2\pi)-n\log\hat{\sigma}_{0}-\frac{n}{2}-(-\frac{n}{2}\log(2\pi)-n\log\hat{\sigma}_{1}-\frac{n}{2}),\\
 & = & n(\log\hat{\sigma}_{1}-\log\hat{\sigma}_{0}).
\end{eqnarray*}
Exponentiate to get 
\[
\frac{l(\hat{\mu}_{0},\hat{\sigma}_{0})}{l(\hat{\mu}_{1},\hat{\sigma}_{1})}=\frac{\hat{\sigma}_{1}^{n}}{\hat{\sigma}_{0}^{n}}=\left(\frac{\hat{\sigma}_{1}^{2}}{\hat{\sigma}_{0}^{2}}\right)^{n/2}=\left(\frac{SSE_{0}}{SSE_{1}}\right)^{-n/2}.
\]
Moreover, since
\[
F=\frac{(SSE_{0}-SSE_{1})/(n-p_{1})}{SSE_{1}/(p_{1}-p_{0})}
\]
we get that
\begin{eqnarray*}
\left(\frac{SSE_{0}}{SSE_{1}}\right)^{-n/2} & = & \left(1+\frac{SSE_{0}-SSE_{1}}{SSE_{1}}\right)^{-n/2},\\
 & = & \left(1+\frac{SSE_{0}-SSE_{1}}{SSE_{1}}\right)^{-n/2}.
\end{eqnarray*}