\section*{Additional Exercise 18}
\subsection*{(a)}

\begin{align*}
f(y) &= \frac{1}{\sigma\sqrt{2\pi y^{3}}}\exp\left[-\frac{1}{2y}\left(\frac{y-\mu}{\mu\sigma}\right)^{2}\right]\\
&= \exp\left[-\frac{1}{2}\left(\frac{y}{\mu^{2}\sigma^{2}} -\frac{2}{\mu\sigma^{2}} + \frac{1}{y\sigma^{2}}\right) -\log\left(\sigma\sqrt{2\pi y^{3}}\right)\right]\\
&= \exp\left[-\frac{1}{2}\left(\frac{y}{\mu^{2}\sigma^{2}} -\frac{2}{\mu\sigma^{2}}\right) -\frac{1}{2y\sigma^{2}} -\log\left(\sigma\sqrt{2\pi y^{3}}\right)\right]\\
&= \exp\left[\frac{-\frac{y}{2\mu^{2}} +\frac{1}{\mu}}{\sigma^{2}} -\frac{1}{2y\sigma^{2}} -\log\left(\sigma\sqrt{2\pi y^{3}}\right)\right]\\
&= \exp\left[\frac{\theta y - b(\theta)}{a(\phi)} + c(y,\phi)\right]
\end{align*}
where $\theta = -\frac{1}{2\mu^{2}}$, $b(\theta) = -\sqrt{-2\theta}  = -\frac{1}{\mu}$, $a(\phi) = \phi = \sigma^{2}$, $c(y,\phi) = -\frac{1}{2y\phi} -\log\left(\sqrt{2\pi y^{3}\phi}\right) = -\frac{1}{2y\sigma^{2}} -\log\left(\sigma\sqrt{2\pi y^{3}}\right)$.\\
So, $f(y)$ is within the exponential dispersion family.\\

\subsection*{(b)}
\begin{align*}
\E[Y] &= b'(\theta) = \frac{1}{\sqrt{-2\theta}} = \mu\\
\Var(Y) &= b''(\theta)a(\phi) = -\frac{-2}{2}(-2\theta)^{-\frac{3}{2}}\phi = (-2\theta)^{-\frac{3}{2}}\phi = \mu^{3}\sigma^{2}\\
\end{align*}


\subsection*{(c)}
Canonical link function $g(\cdot)$ is a link function such that $\theta = g\left(\E[Y] \right)$. (p.123 of the book).
\begin{align*}
\theta = -\frac{1}{2\mu^{2}} = g(\mu)
\end{align*}
Thus, the canonical link function for inverse Gaussian distribution is $g(\mu) = -\frac{1}{2\mu^{2}}$.

\subsection*{(d)}
The log-likelihood function is
\begin{align*}
L(\bm{y},\widehat{\bm{\mu}},\bm{\sigma}^{2}) &= -\frac{1}{2}\sum_{i=1}^{n}\log\left(2\pi\sigma^{2}y_{i}^{3}\right) -\frac{1}{2}\sum_{i=1}^{n}\frac{1}{y_{i}}\left(\frac{y_{i}-\mu_{i}}{\mu_{i}\sigma}\right)^{2}.
\end{align*}
So, the scaled deviance is
\begin{align*}
\frac{D(\bm{y},\widehat{\bm{\mu}})}{\phi} &= -2\left(L\left(\widehat{\bm{\mu}},\bm{y}\right) - L\left(\bm{y},\bm{y}\right)\right)\\
&= -2\left(-\frac{1}{2}\sum_{i=1}^{n}\log\left(2\pi\sigma^{2}y_{i}^{3}\right) -\frac{1}{2}\sum_{i=1}^{n}\frac{1}{y_{i}}\left(\frac{y_{i}-\widehat{\mu}_{i}}{\widehat{\mu}_{i}\sigma}\right)^{2} + \frac{1}{2}\sum_{i=1}^{n}\log\left(2\pi\sigma^{2}y_{i}^{3}\right)\right)\\
&= \sum_{i=1}^{n}\frac{1}{y_{i}}\left(\frac{y_{i}-\widehat{\mu}_{i}}{\widehat{\mu}_{i}\sigma}\right)^{2}\\
&= \frac{1}{\sigma^{2}}\sum_{i=1}^{n}\frac{1}{y_{i}}\left(\frac{y_{i}-\widehat{\mu}_{i}}{\widehat{\mu}_{i}}\right)^{2}.\\
\end{align*}
Hence, the deviance is
\begin{align*}
D(\bm{y},\widehat{\bm{\mu}}) = \sum_{i=1}^{n}\frac{1}{y_{i}}\left(\frac{y_{i}-\widehat{\mu}_{i}}{\widehat{\mu}_{i}}\right)^{2}.
\end{align*}
