\section*{Exercise 5.2}

According note 1.5 on page 21, Hoaglin's partial effect measure for
$\beta_{j}$ is

\[
e_{i}=\frac{1}{n}\sum_{i=1}^{n}\frac{\partial\hat{\mu}_{i}}{\partial x_{ij}}.
\]
In our case, $\hat{\mu}_{i}=\hat{\pi}_{i}$. Recall that 
\[
\hat{\pi}=\frac{1}{1+\exp\left(-\hat{\beta}^{T}x_{i}\right)}
\]
and we can calculate

\begin{eqnarray*}
e_{j} & = & \frac{1}{n}\sum_{i=1}^{n}\frac{\partial\hat{\pi}_{i}}{\partial x_{ij}}\\
 & = & \frac{1}{n}\sum_{i=1}^{n}\frac{\partial}{\partial x_{ij}}\frac{1}{1+\exp\left(-\hat{\beta}^{T}x_{i}\right)},\\
 & = & \hat{\beta}_{j}\frac{1}{n}\sum_{i=1}^{n}\frac{\exp\left(-\hat{\beta}^{T}x_{i}\right)}{\left(\exp\left(-\hat{\beta}^{T}x_{i}\right)+1\right)^{2}},\\
 & = & \hat{\beta}_{j}\frac{1}{n}\sum_{i=1}^{n}\hat{\pi}_{i}(1-\hat{\pi}_{i}).
\end{eqnarray*}
