\section*{Exercise 4.20}
The pmf of Poisson distribution is
\begin{align*}
f(y) = \frac{\mu^{y}}{y!}e^{-\mu}
\end{align*}
So,
\begin{align*}
L(\bm{y}) &= \log\mu\sum_{i=1}^{n}y_{i} - n\mu -\sum_{i}^{n}\log y_{i}!\\
\frac{\partial L(\bm{y})}{\partial \mu} &= \frac{1}{\mu}\sum_{i=1}^{n}y_{i} -n = -n +\frac{n\overline{y}}{\mu}\\
H &= \frac{\partial^{2} L(\bm{y})}{\partial \mu^{2}} = -\frac{n\overline{y}}{\mu^{2}}\\
\mathcal{J} &= \E\left[-\frac{\partial^{2} L(\bm{Y})}{\partial \mu^{2}}\right] = \frac{n}{\mu^{2}}\E\left[\overline{Y}\right] = \frac{n}{\mu}.
\end{align*}

Fisher scoring gives
\begin{align*}
\mu^{(t+1)} = \mu^{(t)} + \left(\mathcal{J}^{(t)}\right)^{-1}u^{(t)} = \mu^{(t)} + \frac{\mu^{(t)}}{n}\left(-n +\frac{n\overline{y}}{\mu^{(t)}}\right) = \overline{y}.
\end{align*}

Newton-Raphson gives
\begin{align*}
\mu^{(t+1)} = \mu^{(t)} + \left(H^{(t)}\right)^{-1}u^{(t)} = \mu^{(t)} -\frac{\left(\mu^{(t)}\right)^{2}}{n\overline{y}}\left(-n +\frac{n\overline{y}}{\mu^{(t)}}\right) = \mu^{(t)}\left(2 - \frac{\mu^{(t)}}{\overline{y}}\right).
\end{align*}
Note that if $\mu^{(t)} = \overline{y}$, then $\mu^{(t+1)} = \overline{y}$.