\section*{Exercise 6.3}
We use vector notation
$\bm{x}_{i} =
\begin{bmatrix}
x_{i,1}, \cdots, x_{i,p}
\end{bmatrix}$
~and~
$\bm{\beta}_{j} =
\begin{bmatrix}
\beta_{j,1}, \cdots, \beta_{j,p}
\end{bmatrix}^{\rm T}$.\\

$\pi_{i,j}$ is defined as
\begin{align*}
\pi_{i,j} =
\begin{cases}
\frac{\exp\left[\bm{x}_{i}\bm{\beta}_{j}\right]}{1+\sum_{h=1}^{c-1}\exp\left[\bm{x}_{i}\bm{\beta}_{h}\right]} ~~&\mbox{for}~~ j = 1, \cdots, c-1\\
\\
\frac{1}{1+\sum_{h=1}^{c-1}\exp\left[\bm{x}_{i}\bm{\beta}_{h}\right]} ~~&\mbox{for}~~ j = c\\
\end{cases}.
\end{align*}
Since the restriction we impose is $\bm{\beta}_{c} = \bm{0}$, I prefer to merge these two cases into one: 
\begin{align*}
\pi_{i,j} =
\frac{\exp\left[\bm{x}_{i}\bm{\beta}_{j}\right]}{\sum_{h=1}^{c}\exp\left[\bm{x}_{i}\bm{\beta}_{h}\right]} ~~&\mbox{for}~~ j = 1, \cdots, c.
\end{align*}

Thus, the rate of change is
\begin{align*}
\frac{\partial \pi_{i,j}}{\partial x_{i,k}} &= \frac{\partial}{\partial x_{i,k}}\left(\frac{\exp\left[\bm{x}_{i}\bm{\beta}_{j}\right]}{\sum_{h=1}^{c}\exp\left[\bm{x}_{i}\bm{\beta}_{h}\right]}\right)\\
&= \frac{\beta_{j,k}\exp\left[\bm{x}_{i}\bm{\beta}_{j}\right] \cdot \sum_{h=1}^{c}\exp\left[\bm{x}_{i}\bm{\beta}_{h}\right] - \exp\left[\bm{x}_{i}\bm{\beta}_{j}\right] \cdot \sum_{h=1}^{c}\beta_{h,k}\exp\left[\bm{x}_{i}\bm{\beta}_{h}\right]}{\left(\sum_{h=1}^{c}\exp\left[\bm{x}_{i}\bm{\beta}_{h}\right]\right)^2}\\
&= \frac{\exp\left[\bm{x}_{i}\bm{\beta}_{j}\right]}{\sum_{h=1}^{c}\exp\left[\bm{x}_{i}\bm{\beta}_{h}\right]}\left(\frac{\beta_{j,k}\sum_{h=1}^{c}\exp\left[\bm{x}_{i}\bm{\beta}_{h}\right] - \sum_{h=1}^{c}\beta_{h,k}\exp\left[\bm{x}_{i}\bm{\beta}_{h}\right]}{\sum_{h=1}^{c}\exp\left[\bm{x}_{i}\bm{\beta}_{h}\right]}\right)\\
&= \frac{\exp\left[\bm{x}_{i}\bm{\beta}_{j}\right]}{\sum_{h=1}^{c}\exp\left[\bm{x}_{i}\bm{\beta}_{h}\right]}\left(\beta_{j,k} -\frac{\sum_{h=1}^{c}\beta_{h,k}\exp\left[\bm{x}_{i}\bm{\beta}_{h}\right]}{\sum_{h=1}^{c}\exp\left[\bm{x}_{i}\bm{\beta}_{h}\right]}\right)\\
&= \frac{\exp\left[\bm{x}_{i}\bm{\beta}_{j}\right]}{\sum_{h=1}^{c}\exp\left[\bm{x}_{i}\bm{\beta}_{h}\right]}\left(\beta_{j,k} -\sum_{h=1}^{c}\left[\frac{\exp\left[\bm{x}_{i}\bm{\beta}_{h}\right]}{\sum_{h=1}^{c}\exp\left[\bm{x}_{i}\bm{\beta}_{h}\right]}\beta_{h,k}\right]\right)\\
&= \pi_{i,j}\left(\beta_{j,k} -\sum_{h=1}^{c}\left[\pi_{i,h}\beta_{h,k}\right]\right)\\
&= \pi_{i,j}\left(\beta_{j,k} -\sum_{h=1}^{c-1}\left[\pi_{i,h}\beta_{h,k}\right]\right)
\end{align*}

In binary case (i.e. $c = 2$), $j = 1$. So, the rate of change simplifies to 
\begin{align*}
\frac{\partial \pi_{i}}{\partial x_{i,k}} = \beta_{k}\pi_{i}(1-\pi_{i}).
\end{align*}
