\section*{Exercise 5.25}

\subsection*{(i)}
With complementary log-log link we have
\begin{align*}
\log\left(-\log(1-\pi_{i})\right) &= \beta_{0} + \beta_{1}x_{i}\\
\log\left(\frac{1}{1-\pi_{i}}\right) &= \exp\left[\beta_{0} + \beta_{1}x_{i}\right]\\
\frac{1}{1-\pi_{i}} &= \exp\left[\exp\left[\beta_{0} + \beta_{1}x_{i}\right]\right]\\
\pi_{i} &= 1 - \frac{1}{\exp\left[\exp\left[\beta_{0} + \beta_{1}x_{i}\right]\right]}\\
\end{align*}

When $\pi_{i} = 0.5$,
\begin{align*}
2 &= \exp\left[\exp\left[\beta_{0} + \beta_{1}x_{i}\right]\right]\\
\log\left(\log 2\right) &= \beta_{0} + \beta_{1}x_{i}\\
x_{i} &= \frac{\log\left(\log 2\right) - \beta_{0}}{\beta_{1}} = \frac{-0.3665 -\beta_{0}}{\beta_{1}}.\\
\end{align*}

The rate of change is
\begin{align*}
\frac{\partial \pi_{i}}{\partial x_{i}} &= \frac{\partial \pi_{i}}{\partial \eta_{i}}\frac{\partial \eta_{i}}{\partial x_{i}}\\
&= \frac{\exp\left[\exp\left[\beta_{0} + \beta_{1}x_{i}\right]\right] \cdot \exp\left[\beta_{0} + \beta_{1}x_{i}\right]}{\left(\exp\left[\exp\left[\beta_{0} + \beta_{1}x_{i}\right]\right]\right)^{2}}\beta_{1}\\
&= \frac{\exp\left[\beta_{0} + \beta_{1}x_{i}\right]}{\exp\left[\exp\left[\beta_{0} + \beta_{1}x_{i}\right]\right]}\beta_{1}.
\end{align*}

We find $x_{i}$ that maximizes the rate of change
\begin{align*}
\frac{\partial^{2} \pi_{i}}{\partial x_{i}^{2}} &= \frac{\partial}{\partial x_{i}}\left(\frac{\partial \pi_{i}}{\partial x_{i}}\right)\\
&= \frac{\partial}{\partial x_{i}}\left(\frac{\exp\left[\beta_{0} + \beta_{1}x_{i}\right]}{\exp\left[\exp\left[\beta_{0} + \beta_{1}x_{i}\right]\right]}\beta_{1}\right)\\
&= \frac{\beta_{1} \exp\left[\beta_{0} + \beta_{1}x_{i}\right]\exp\left[\exp\left[\beta_{0} + \beta_{1}x_{i}\right]\right] - \exp\left[\beta_{0} + \beta_{1}x_{i}\right] \exp\left[\exp\left[\beta_{0} + \beta_{1}x_{i}\right]\right] \exp\left[\beta_{0} + \beta_{1}x_{i}\right] \beta_{1}}{\left(\exp\left[\exp\left[\beta_{0} + \beta_{1}x_{i}\right]\right]\right)^{2}}\beta_{1}\\
&= \frac{\exp\left[\beta_{0} + \beta_{1}x_{i}\right] - \exp\left[\beta_{0} + \beta_{1}x_{i}\right] \exp\left[\beta_{0} + \beta_{1}x_{i}\right] }{\exp\left[\exp\left[\beta_{0} + \beta_{1}x_{i}\right]\right]}\beta_{1}^{2}\\
&= \frac{\exp\left[\beta_{0} + \beta_{1}x_{i}\right]\left(1 - \exp\left[\beta_{0} + \beta_{1}x_{i}\right]\right)}{\exp\left[\exp\left[\beta_{0} + \beta_{1}x_{i}\right]\right]}\beta_{1}^{2}\\
&= 0.
\end{align*}
So, the rate of change reaches its maximum when $\exp\left[\beta_{0} + \beta_{1}x_{i}\right] = 1$. We have then $\beta_{0} + \beta_{1}x_{i} = 0$ and $x_{i} = -\frac{\beta_{0}}{\beta_{1}}$. When $x_{i} = -\frac{\beta_{0}}{\beta_{1}}$, $\pi_{i} = 1 - \frac{1}{e} = 0.6321$.\\

\subsection*{(ii)}
Repeat i) for log-log link
\begin{align*}
-\log\left(-\log\pi_{i}\right) &= \beta_{0} + \beta_{1}x_{i}\\
\end{align*}